@prefix : <http://www.semanticweb.org/dggrs/> .
@prefix owl: <http://www.w3.org/2002/07/owl#> .
@prefix rdf: <http://www.w3.org/1999/02/22-rdf-syntax-ns#> .
@prefix xml: <http://www.w3.org/XML/1998/namespace> .
@prefix xsd: <http://www.w3.org/2001/XMLSchema#> .
@prefix rdfs: <http://www.w3.org/2000/01/rdf-schema#> .
@prefix geosrs: <https://w3id.org/geosrs> .
@base <http://www.semanticweb.org/dggrs/> .

<http://www.semanticweb.org/dggrs> rdf:type owl:Ontology ;
        rdfs:label "Discrete Global Grid Reference Systems ontology"@en ;
        rdfs:comment """A means to express and record Discrete Global Grid 
                        Reference Systems on the web. This ontology depends on 
                        the CRS ontology in development at the OGC."""@en ;
        rdf:seeAlso geosrs: ;
        dcterms:license <https://creativecommons.org/licenses/by-nc-nd/4.0/> ;
        dcterms:rights "This ontology is distributed under Attribution-NonCommercial-NoDerivs 4.0 International License"@en ;
        dcterms:creator 
            [ rdfs:seeAlso <http://orcid.org/0000-0002-5851-2071> ;
              foaf:name "Luís Moreira de Sousa" ] .

#################################################################
#    Classes
#################################################################

:DGGRS rdf:type owl:Class ; 
       rdfs:subClassOf geosrs:SpatialReferenceSystem ;
       rdfs:label "Discrete Global Grid Reference System (DGGRS)"@en ;
       rdfs:comment """A Spatial Reference System composed of a Discrete Global 
                       Grid System and a zone (cell) indexing mechanism allowing 
                       for discrete but precise location on the surface of the 
                       Earth."""@en .

:Polyhedron rdf:type owl:Class ; 
       rdfs:label "Polyhedron"@en ;
       rdfs:comment """A multi-faceted solid providing a geometric structure to 
                       divide a sphere or ellipsoid. The platonic solids are 
                       the most commonly used, although alternatives may also 
                       be used, such as the truncated icosahedron."""@en .

:Index rdf:type owl:Class ; 
       rdfs:label "DGGRS indexing mechanism"@en ;
       rdfs:comment """A mathematical function, ordering mechanism, or any other 
                       method providing a unique identifier to each zone (cell) 
                       of a DGGRS, at any refinement level (resolution)."""@en .

:ImplDGGRS rdf:type owl:Class ; 
       rdfs:label "DGGRS implementation"@en ;
       rdfs:comment """A software system implementing a DGGRS. It should at a minimum provide an API to transform a geographic location into a zone (cell) identifier at a given refinement level (resolution), plus its inverse. """@en .

#################################################################
#    Object Properties
#################################################################

:basePolyhedron rdf:type owl:ObjectProperty ;
        rdfs:label "Base polyhedron of a DGGRS"@en ;
        rdfs:comment """Usually a polyhedron on which faces the datum 
                      surface is projected for further sub-division."""@en ; 
        rdfs:domain :DGGRS ;
        rdfs:range :Polyhedron .

:usesIndex rdf:type owl:ObjectProperty ;
        rdf:label "Indexing mechanism used in a DGGRS"@en ;
        rdf:comment """Indicates that a particular software software system 
                       implements a known DGGRS"""@en ;
        rdfs:domain :DGGRS ;
        rdfs:range :Index .  

:implements rdf:type owl:ObjectProperty ;
        rdf:label "Implementation of a DGGRS"@en ;
        rdf:comment """Indicates that a particular software software system 
                       implements a known DGGRS"""@en ;
        rdfs:domain :ImplDGGRS ;
        rdfs:range :DGGRS .  

#################################################################
#    DataType Properties
#################################################################


:zoneShape rdf:type owl:DatatypeProperty ;
         rdfs:label "Shape of zones (cells) in a DGGRS"@en ;
         rdfs:comment """Usually a regular shape like the hexagon or triangle. 
                         May also be a rhombic shape such as the parellelogram."""@en ; 
         rdfs:domain :DGGRS ;
         rdfs:range xsd:string .

:aperture rdf:type owl:DatatypeProperty ;
    rdfs:label "DGGRS zone sub-division aperture"@en ;
    rdfs:comment """The number of zones in the subsequent DGGRS refinement 
                    level corresponding to a zone on the current level. Rate 
                    of zone sub-division. The higher the number, the ´faster' 
                    a DGGRS refines to small zones."""@en ;
    rdfs:domain :DGGRS ;
    rdfs:range [
        rdf:type rdfs:Datatype;
        owl:onDatatype  xsd:integer;
        owl:withRestrictions ( [xsd:minInclusive 2] )
    ] .


#################################################################
#    Individuals
#################################################################

:tetrahedron rdf:type :Polyhedron ;
        rdfs:label "Tetrahedron"@en ;
        rdfs:comment """A solid with four equal faces which are equilateral 
                           triangles."""@en .

:hexahedron rdf:type :Polyhedron ;
        rdfs:label "Hexahedron"@en ;
        rdfs:comment """A solid with six equal faces which are squares"""@en . 

:dodecahedron rdf:type :Polyhedron ;
        rdfs:label "Dodecahedron"@en ;
        rdfs:comment """A solid with twelve equal faces which are pentagons."""@en .

:icosahedron rdf:type :Polyhedron ;
        rdfs:label "Icosahedron"@en ;
        rdfs:comment """A solid with twenty equal faces which are equilateral 
                           triangles."""@en .

:gbt rdf:type :Index ;
        rdfs:label "Generalised Balanced Trenary"@en ;
        rdfs:comment """Indexes hexagonal grid systems of aperture 7. At 
                           each refinement level cells rotate circa 20º so that 
                           vertices of a cell septet concide with the six 
                           vertices of a cell in the previous refinement level."""@en ;
        rdfs:seeAlso <https://en.wikipedia.org/wiki/Generalized_balanced_ternary> .

:z7 rdf:type :Index ;
        rdfs:label "Z7"@en ;
        rdfs:comment """An index for hexagonal grid systems of aperture 7."""@en ; 
        rdfs:seeAlso <http://dx.doi.org/10.5194/agile-giss-6-32-2025> .

:9r rdf:type :Index ;
        rdfs:label "9R"@en ;
        rdfs:comment """A highly compact index for hexagonal grid systems 
                        developed by Ecere and first implemented by DGGAL."""@en .


